src/tls/HMAC.UFCMA.fst
@@ -30,7 +30,7 @@ type ha = Hashing.alg
 // initial parameters
 noeq type info = | Info: 
   parent: rgn {~ (is_tls_rgn parent)} -> 
-  alg: Hashing.alg -> //too loose? Pkg.kdfa;
+  alg: HMAC.ha -> 
   good: (Hashing.macable alg -> bool) ->  //TODO: should be Type0 instead of bool, and erased, but hard to propagate
   info
 
@@ -299,7 +299,7 @@ private let ip : ipkg = Pkg.Idx id (fun _ -> True) (fun _ -> True) (fun _ -> tru
 #set-options "--initial_fuel 1 --max_fuel 1 --initial_ifuel 1 --max_ifuel 1 --z3rlimit 10"
 
 noextract
-private let test (a: ha) (r: rgn{~(is_tls_rgn r)}) (v': Hashing.macable a) (t': Hashing.Spec.tag a)
+private let test (a: HMAC.ha) (r: rgn{~(is_tls_rgn r)}) (v': Hashing.macable a) (t': Hashing.Spec.tag a)
   : ST bool
   (requires fun h0 -> model)
   (ensures fun h0 _ h1 -> True)
